\documentclass[a4paper, twocolumn]{article}
\setlength{\oddsidemargin}{0cm}
\setlength{\evensidemargin}{0cm}
\setlength{\topmargin}{0cm}
\usepackage{indentfirst}
\usepackage[utf8]{inputenc}

\begin{document}

\section{Statistische Maßzahlen}

    empirische Kovarianz
    \begin{displaymath}
        \tilde{s}_{xy} = \frac{1}{n-1} \sum^n_{i=1} (x_{i}-\bar{x}) (y_{i}-\bar{y})
    \end{displaymath} \\
    
    empirische Varianz:
    \begin{displaymath}
      \sigma^2 = \tilde{s}^2 = \tilde{s}^2_x := 
      \frac{1}{n-1} \sum^{n}_{i=1} (x_{i} - \bar{x})^2 = \frac{1}{n-1}(\sum^n_{i=1} x^2_i -n \bar x^2)
    \end{displaymath} \\
    
    Standardabweichung
    \begin{displaymath}
      \sigma = \tilde s = \tilde s_x = \sqrt{\tilde s ^2}
    \end{displaymath} \\
    
    empirischer Korrelationskoeffizient (nach Bravais Pearson)
    \begin{displaymath}
     r_{xy} = \frac{\tilde s_{xy}}{\tilde s_x \cdot \tilde s_y}
    \end{displaymath} \\
    
    
    Spearman'sche Rangkorrelationskoeffizient von X und Y
    \begin{equation}
      r_{SP}(x,y) = \frac
      {\sum\limits^n_{i=1} \Big(rg(x_i) - \overline{rg_x}) (rg(y_i)- \overline{rg_y} \Big) }
      { \sqrt{ \sum\limits^n_{i=1} (rg(x_i) - \bar{rg_x})^2 \cdot \sum\limits^n_{i=1} (rg(y_i) - \bar{rg_y})^2 }}
    \end{equation}
    
    \subsection{Lineare Regression}
        optimale Ausgleichgerade:
        \begin{displaymath}
            y = f(x) = \hat a x + \hat b
        \end{displaymath}
        
        \begin{displaymath}
            \hat a = \frac{\tilde s_{xy}}{\tilde s^2_x}
        \end{displaymath}
        
        \begin{displaymath}
            \hat b = \bar y - \hat a \bar x
        \end{displaymath}
        
        Bestimmtheitsmaß, Modellgüte:
        \begin{displaymath}
          R^2 = r^2_{xy}
        \end{displaymath}
        
\section{Wahrscheinlichkeit}
	es gilt:\\
		$ P(A \cap B) = P(A) + P(B) - P(A \cup B)  $ \\
		$ P(A \cup B) = P(A) + P(B) - P(A \cap B) $ \\
		$ P(A \cap \overline B) = P(A) - P(A \cap B) $ \\
		$ P(\overline A  \cap \overline B) = P(\overline{A \cup B}) = 1 - P(A \cup B) $






\end{document}
    